---
layout: post
title: leetcode - [509] Fibonacci Number
category: algorithm
tags: [algorithm]
excerpt: Fibonacci Number
---

## 题目描述  

> The Fibonacci numbers, commonly denoted F(n) form a sequence, called the Fibonacci sequence, such that each number is the sum of the two preceding ones, starting from 0 and 1.  

> 0 ≤ N ≤ 30.  

直接举个例子：  

``` java
Input: 2
Output: 1
Explanation: F(2) = F(1) + F(0) = 1 + 0 = 1.

Input: 3
Output: 2
Explanation: F(3) = F(2) + F(1) = 1 + 1 = 2.

Input: 4
Output: 3
Explanation: F(4) = F(3) + F(2) = 2 + 1 = 3.
```

![](https://yyc-images.oss-cn-beijing.aliyuncs.com/leetcode_509_fibonacci.png)


## Update at 2020_0604  

本题可以使用`DP[动态规划]`思想：  

![](https://yyc-images.oss-cn-beijing.aliyuncs.com/leetcode_509_using_dp.png)

来看下实现：  


``` java
class Solution {
    public int fib(int N) {
        // Corner case.
        if (N == 0) return 0;

        // Initilization dp.
        int[] dp = new int[N + 1];
        dp[1] = 1;

        for (int i = 2; i <= N; i++){
            // formula
            dp[i] = dp[i - 1] + dp[i - 2];
        }

        return dp[N];
    }
}
```

然后再简化成两个变量：  

``` java
class Solution {
    public int fib(int N) {
        if (N == 0) return 0;
        int pre = 0;
        int cur = 1;
        
        for (int i = 2; i <= N; i++){
            int tmp = cur;
            cur += pre;
            pre = tmp;
        }
        return cur;
    }
}
```

`Enjoy it ! `

## 解法1  

这道题和 [70. Climbing Stairs](http://yaoyichen.cn/algorithm/2020/04/05/leetcode-70.html){:target="_blank"} 的思路是一致的：  

Thanks [@StefanPochmann](https://leetcode.com/problems/climbing-stairs/discuss/25296/3-4-short-lines-in-every-language){:target="_blank"}  again!


``` java
class Solution {
    public int fib(int N) {
        int a = 0, b = 1;
        while (N-- > 0){
            int tmp = b;
            b += a;
            a = tmp;
        }
        return a;
    }
}
```

优化：  

``` java
class Solution {
    public int fib(int N) {
        int a = 0, b = 1;
        while (N-- > 0){
            a = (b += a) - a;
        }
        return a;
    }
}
```
